thys/Pi_Calculus/Pi_Transition_Common.thy
@@ -1,0 +1,84 @@
+theory Pi_Transition_Common
+  imports Commitment
+begin
+
+hide_const inverse_class.inverse_divide
+no_notation inverse.inverse_divide (infixl "'/" 70)
+
+type_synonym T = "trm \<times> cmt"
+type_synonym V = "var list" 
+
+fun Tperm :: "(var \<Rightarrow> var) \<Rightarrow> T \<Rightarrow> T" where 
+"Tperm f = map_prod (rrename f) (rrename_commit f)"
+
+fun Tsupp :: "T \<Rightarrow> var set" where 
+"Tsupp (e1,e2) = FFVars e1 \<union> FFVars_commit e2"
+
+(* Supply of fresh variables: *)
+lemma finite_Tsupp: "finite (Tsupp t)"
+  by (metis FFVars_commit_simps(5) Tsupp.elims finite_FFVars_commit finite_Un)
+
+lemma exists_fresh:
+"\<exists> z. z \<notin> set xs \<and> (\<forall>t \<in> set ts. z \<notin> Tsupp t)"
+proof-
+  have 0: "|set xs \<union> \<Union> (Tsupp ` (set ts))| <o |UNIV::var set|" 
+  unfolding ls_UNIV_iff_finite  
+  using finite_Tsupp by blast
+  then obtain x where "x \<notin> set xs \<union> \<Union> (Tsupp ` (set ts))"
+  by (meson ex_new_if_finite finite_iff_le_card_var 
+    infinite_iff_natLeq_ordLeq var_term_pre_class.large)
+  thus ?thesis by auto
+qed
+
+lemma finite_vars: "finite (vars act)"
+  by (cases act) auto
+
+lemma exists_fresh':
+"\<exists> z. z \<notin> set xs \<and> (\<forall>t \<in> set as. z \<notin> vars t) \<and> (\<forall>t \<in> set ts. z \<notin> Tsupp t)"
+proof-
+  have 0: "|set xs \<union> \<Union> (Tsupp ` (set ts)) \<union> \<Union> (vars ` (set as))| <o |UNIV::var set|" 
+  unfolding ls_UNIV_iff_finite
+  using finite_Tsupp finite_vars by blast
+  then obtain x where "x \<notin> set xs \<union> \<Union> (Tsupp ` (set ts)) \<union> \<Union> (vars ` (set as))"
+  by (meson ex_new_if_finite finite_iff_le_card_var 
+    infinite_iff_natLeq_ordLeq var_term_pre_class.large)
+  thus ?thesis by auto
+qed
+
+ML \<open>fun gen_fresh ctxt xs0 acts0 ts0 = HEADGOAL (Subgoal.FOCUS_PARAMS (fn {context = ctxt, params = cps, ...} =>
+  let
+    val ps = map (Thm.term_of o snd) cps;
+    fun mk zs T = filter (fn t => fastype_of t = T) ps |> append zs |> HOLogic.mk_list T |> Thm.cterm_of ctxt;
+    val xs = mk xs0 @{typ var};
+    val acts = mk acts0 @{typ "var action"};
+    val ts = mk ts0 @{typ "var term * var commit"};
+    val thm = infer_instantiate' ctxt [SOME xs, SOME acts, SOME ts] @{thm exists_fresh'} RS exE;
+  in HEADGOAL (resolve_tac ctxt [thm]) end) ctxt)\<close>
+
+lemma isPerm_swap: "isPerm (id(x := y, y := x))"
+  by (auto simp: isPerm_def MRBNF_FP.supp_swap_bound infinite_UNIV)
+
+lemma R_forw_subst: "R (x, y) \<Longrightarrow> (\<And>x y. R (x, y) \<Longrightarrow> R (f x, g y)) \<Longrightarrow> z = g y \<Longrightarrow> R (f x, z)"
+  by blast
+
+lemma FFVars_commit_Cmt: "FFVars_commit (Cmt act P) = fvars act \<union> (FFVars P - bvars act)"
+  by (cases act) auto
+
+lemma empty_bvars_vars_fvars: "bvars act = {} \<Longrightarrow> vars act = fvars act"
+  by (cases act) auto
+
+lemma bvars_swapa: "bvars act = {} \<Longrightarrow> bvars (swapa act x xx) = {}"
+  by (cases act) auto
+
+lemma fvars_swapa: "xx \<in> fvars (swapa act x xx) \<longleftrightarrow> x \<in> fvars act"
+  by (cases act) auto
+
+lemma swapa_idle: "xx \<notin> vars act \<Longrightarrow> x \<notin> vars act \<Longrightarrow> swapa act x xx = act"
+  by (cases act) auto
+
+lemmas act_var_simps = empty_bvars_vars_fvars bvars_swapa fvars_swapa swapa_idle
+
+lemma small_bns[simp]: "small (bns \<alpha>)"
+  by (cases \<alpha>) auto
+
+end
