thys/Pi_Calculus/Pi_Transition_Late.thy
@@ -1,11 +1,11 @@
-theory Pi_Transition_Early
+theory Pi_Transition_Late
   imports Pi_Transition_Common
 begin
 
 binder_inductive trans :: "trm \<Rightarrow> cmt \<Rightarrow> bool" where
-  InpE: "trans (Inp a x P) (Finp a y (P[y/x]))" binds "{x}"
-| ComLeftE: "\<lbrakk> trans P (Finp a x P') ; trans Q (Fout a x Q') \<rbrakk> \<Longrightarrow> trans (P \<parallel> Q) (Tau (P' \<parallel> Q'))"
-| CloseLeftE: "\<lbrakk> trans P (Finp a x P') ; trans Q (Bout a x Q') ; x \<notin> {a} \<union> FFVars P \<rbrakk> \<Longrightarrow> trans (P \<parallel> Q) (Tau (Res x (P' \<parallel> Q')))" binds "{x}"
+  InpL: "trans (Inp a x P) (Binp a x P)" binds "{x}"
+| ComLeftL: "\<lbrakk> trans P (Binp a x P') ; trans Q (Fout a x Q') \<rbrakk> \<Longrightarrow> trans (P \<parallel> Q) (Tau ((P'[y/x]) \<parallel> Q'))" binds "{x}"
+| CloseLeftL: "\<lbrakk> trans P (Binp a x P') ; trans Q (Bout a x Q') \<rbrakk> \<Longrightarrow> trans (P \<parallel> Q) (Tau (Res x (P' \<parallel> Q')))" binds "{x}"
 | Open: "\<lbrakk> trans P (Fout a x P') ; a \<noteq> x \<rbrakk> \<Longrightarrow> trans (Res x P) (Bout a x P')" binds "{x}"
 | ScopeFree: "\<lbrakk> trans P (Cmt \<alpha> P') ; fra \<alpha> ; x \<notin> ns \<alpha> \<rbrakk> \<Longrightarrow> trans (Res x P) (Cmt \<alpha> (Res x P'))" binds "{x}"
 | ScopeBound: "\<lbrakk> trans P (Bout a x P') ; y \<notin> {a, x} ; x \<notin> FFVars P \<union> {a} \<rbrakk> \<Longrightarrow> trans (Res y P) (Bout a x (Res y P'))" binds "{x,y}"
@@ -36,4 +36,4 @@ apply (auto simp: o_def split_beta term.rrename_comps fun_eq_iff isPerm_def
     sorry
   done
 
-
+end
